SoftwareFoundations/LogicalFoundations/AltAuto.lean
@@ -1,0 +1,3 @@
+/-
+# A Streamlined Treatment of Automation
+-/
