SoftwareFoundations/LogicalFoundations/Auto.lean
@@ -1,0 +1,3 @@
+/-
+# More Automation
+-/
