SoftwareFoundations/LogicalFoundations/Extraction.lean
@@ -1,0 +1,3 @@
+/-
+# Extracting OCaml from Coq
+-/
