SoftwareFoundations/LogicalFoundations/Imp.lean
@@ -1,0 +1,714 @@
+/-
+# Simple Imperative Programs
+-/
+
+import «SoftwareFoundations».«LogicalFoundations».«Maps»
+import Mathlib.tactic.linarith
+
+/-
+## Arithmetic and Boolean Expressions
+-/
+
+/-
+### Syntax
+-/
+
+namespace AExp
+  inductive Arith: Type where
+    | num (n: Nat): Arith
+    | plus (e₁ e₂: Arith): Arith
+    | minus (e₁ e₂: Arith): Arith
+    | mult (e₁ e₂: Arith): Arith
+
+  def Arith.eval: Arith → Nat
+    | .num n => n
+    | .plus e₁ e₂ => e₁.eval + e₂.eval
+    | .minus e₁ e₂ => e₁.eval - e₂.eval
+    | .mult e₁ e₂ => e₁.eval * e₂.eval
+
+  def Arith.optZeroPlus: Arith → Arith
+    | .num n => .num n
+    | .plus (.num 0) e₂ => e₂.optZeroPlus
+    | .plus e₁ e₂ => .plus e₁.optZeroPlus e₂.optZeroPlus
+    | .minus e₁ e₂ => .minus e₁.optZeroPlus e₂.optZeroPlus
+    | .mult e₁ e₂ => .mult e₁.optZeroPlus e₂.optZeroPlus
+
+  example: (Arith.plus (.num 2) (.num 2)).eval = 4 := rfl
+  example: (Arith.plus (.num 2) (.plus (.num 0) (.plus (.num 0) (.num 1)))).optZeroPlus = .plus (.num 2) (.num 1) := rfl
+
+  theorem Arith.optZeroPlus.sound (a: Arith): a.optZeroPlus.eval = a.eval := by
+    induction a with
+      | num n => rfl
+      | plus e₁ e₂ ih₁ ih₂ =>
+        cases e₁ with
+          | num n =>
+            cases n with
+              | zero => sorry
+              | succ n => sorry
+          | plus e₃ e₄ =>
+            unfold optZeroPlus eval
+            rw [ih₁, ih₂]
+          | minus e₃ e₄ =>
+            unfold optZeroPlus eval
+            rw [ih₁, ih₂]
+          | mult e₃ e₄ =>
+            unfold optZeroPlus eval
+            rw [ih₁, ih₂]
+      | minus e₁ e₂ ih₁ ih₂ =>
+        unfold optZeroPlus eval
+        rw [ih₁, ih₂]
+      | mult e₁ e₂ ih₁ ih₂ =>
+        unfold optZeroPlus eval
+        rw [ih₁, ih₂]
+
+  inductive Logic: Type where
+    | true: Logic
+    | false: Logic
+    | eq (e₁ e₂: Arith): Logic
+    | neq (e₁ e₂: Arith): Logic
+    | le (e₁ e₂: Arith): Logic
+    | gt (e₁ e₂: Arith): Logic
+    | not (e: Logic): Logic
+    | and (e₁ e₂: Logic): Logic
+
+  def Logic.eval: Logic → Bool
+    | .true => Bool.true
+    | .false => Bool.false
+    | .eq e₁ e₂ => e₁.eval == e₂.eval
+    | .neq e₁ e₂ => e₁.eval != e₂.eval
+    | .le e₁ e₂ => e₁.eval ≤ e₂.eval
+    | .gt e₁ e₂ => e₁.eval > e₂.eval
+    | .not e => !e.eval
+    | .and e₁ e₂ => e₁.eval && e₂.eval
+
+  def Logic.optZeroPlus: Logic → Logic
+    | .true => .true
+    | .false => .false
+    | .eq e₁ e₂ => .eq e₁.optZeroPlus e₂.optZeroPlus
+    | .neq e₁ e₂ => .neq e₁.optZeroPlus e₂.optZeroPlus
+    | .le e₁ e₂ => .le e₁.optZeroPlus e₂.optZeroPlus
+    | .gt e₁ e₂ => .gt e₁.optZeroPlus e₂.optZeroPlus
+    | .not e => .not e.optZeroPlus
+    | .and e₁ e₂ => .and e₁.optZeroPlus e₂.optZeroPlus
+
+  /-
+  ## Lean (Coq) Automation
+  -/
+
+  /-
+  ### The `try` Tactical
+  -/
+
+  example (P: Prop) (h: P): P := by
+    try rfl
+    apply h
+
+  example (a: Arith): a.eval = a.eval := by
+    try rfl
+
+  /-
+  ### The `<;>` Tactical (Simple Form)
+  -/
+
+  example (n: Nat): 0 ≤ n := by
+    cases n with
+      | zero => simp
+      | succ n => simp
+
+  example (n: Nat): 0 ≤ n := by
+    cases n <;> simp
+
+  /-
+  ### The `<;>` Tactical (General Form)
+  -/
+
+  example (a: Arith): a.optZeroPlus.eval = a.eval := by
+    induction a
+    try rfl
+    case minus e₁ e₂ ih₁ ih₂ | mult e₁ e₂ ih₁ ih₂ =>
+      unfold Arith.optZeroPlus Arith.eval
+      rw [ih₁, ih₂]
+    case plus e₁ _ ih₁ ih₂ =>
+      cases e₁ <;>
+      try (unfold Arith.optZeroPlus Arith.eval; rw [ih₁, ih₂])
+      case num n =>
+        cases n with
+          | zero => sorry
+          | succ n => sorry
+
+  /-
+  ### The `repeat` Tactical
+  -/
+
+  def In (x: α) (l: List α): Prop :=
+    match l with
+      | [] => False
+      | b :: m => b = x \/ In x m
+
+  example: In 10 [1, 2, 3, 4, 5, 6, 7, 8, 9, 10] := by
+    repeat (try (first | apply Or.inl; rfl | apply Or.inr))
+
+  theorem Logic.optZeroPlus.sound (e: Logic): e.optZeroPlus.eval = e.eval := by
+    induction e <;>
+    try (first | rfl
+               | unfold Logic.optZeroPlus Logic.eval
+                 simp [Arith.optZeroPlus.sound])
+    case not e ih =>
+      unfold Logic.optZeroPlus Logic.eval
+      rw [ih]
+    case and e₁ e₂ ih₁ ih₂ =>
+      unfold Logic.optZeroPlus Logic.eval
+      rw [ih₁, ih₂]
+
+  -- TODO: Moar optimization
+
+  /-
+  ## Defining New Tactics
+  -/
+
+  -- TODO: Research defining tactics in Lean
+
+  /-
+  ## The `linearith` (`lia`) Tactic
+  -/
+
+  -- import Mathlib.tactics.linarith
+
+  example (n₁ n₂ n₃ n₄: Nat) (h: n₁ + n₂ ≤ n₂ + n₃ ∧ n₃ + 3 = n₄ + 3): n₁ ≤ n₄ := by
+    linarith
+
+  example (n₁ n₂: Nat): n₁ + n₂ = n₂ + n₁ := by
+    linarith
+
+  example (n₁ n₂ n₃: Nat): n₁ + (n₂ + n₃) = (n₁ + n₂) + n₃ := by
+    linarith
+
+  /-
+  ## A Few More Handy Tactics
+  -/
+
+  -- TODO: Research the same tactics in Lean
+
+  /-
+  ## Evaluation as a Relation
+  -/
+
+  inductive ArithEval: Arith → Nat → Prop where
+    | num (n: Nat): ArithEval (.num n) n
+    | plus (e₁ e₂: Arith) (n₁ n₂: Nat) (h₁: ArithEval e₁ n₁) (h₂: ArithEval e₂ n₂): ArithEval (.plus e₁ e₂) (n₁ + n₂)
+    | minus (e₁ e₂: Arith) (n₁ n₂: Nat) (h₁: ArithEval e₁ n₁) (h₂: ArithEval e₂ n₂): ArithEval (.minus e₁ e₂) (n₁ - n₂)
+    | mult (e₁ e₂: Arith) (n₁ n₂: Nat) (h₁: ArithEval e₁ n₁) (h₂: ArithEval e₂ n₂): ArithEval (.mult e₁ e₂) (n₁ * n₂)
+
+  /-
+  ### Inference Rule Notation
+  -/
+
+  inductive LogicEval: Logic → Bool → Prop where
+    | true: LogicEval .true true
+    | false: LogicEval .false false
+    | eq (e₁ e₂: Arith) (n₁ n₂: Nat) (h₁: ArithEval e₁ n₁) (h₂: ArithEval e₂ n₂): LogicEval (.eq e₁ e₂) (n₁ == n₂)
+    | neq (e₁ e₂: Arith) (n₁ n₂: Nat) (h₁: ArithEval e₁ n₁) (h₂: ArithEval e₂ n₂): LogicEval (.neq e₁ e₂) (n₁ != n₂)
+    | le (e₁ e₂: Arith) (n₁ n₂: Nat) (h₁: ArithEval e₁ n₁) (h₂: ArithEval e₂ n₂): LogicEval (.neq e₁ e₂) (n₁ ≤ n₂)
+    | gt (e₁ e₂: Arith) (n₁ n₂: Nat) (h₁: ArithEval e₁ n₁) (h₂: ArithEval e₂ n₂): LogicEval (.neq e₁ e₂) (n₁ > n₂)
+    | not (e: Logic) (b: Bool) (h: LogicEval e b): LogicEval (.not e) !b
+    | and (e₁ e₂: Logic) (b₁ b₂: Bool) (h₁: LogicEval e₁ b₁) (h₂: LogicEval e₂ b₂): LogicEval (.and e₁ e₂) (b₁ && b₂)
+
+  /-
+  ### Equivalence of Definitions
+  -/
+
+  theorem arith_eval_eval (a: Arith) (n: Nat): ArithEval a n ↔ a.eval = n := by
+    apply Iff.intro
+    · intro h
+      induction h <;> first | rfl
+                            | unfold Arith.eval
+                              simp_all
+    · intro h₁
+      induction a with
+        | num n =>
+          rw [← h₁]
+          exact ArithEval.num n
+        | plus e₁ e₂ ih₁ ih₂ =>
+          unfold Arith.eval at h₁
+          sorry
+        | _ => sorry
+
+  theorem logic_eval_eval (l: Logic) (b: Bool): LogicEval l b ↔ l.eval = b := by
+    apply Iff.intro
+    · intro h
+      induction h with
+        | true => rfl
+        | false => rfl
+        | eq e₁ e₂ n₁ n₂ h₁ h₂ =>
+          unfold Logic.eval
+          sorry
+        -- Other Arith cases
+        | not e b h ih =>
+          unfold Logic.eval
+          rw [ih]
+        | and e₁ e₂ b₁ b₂ h₁ h₂ ih₁ ih₂ =>
+          unfold Logic.eval
+          rw [ih₁, ih₂]
+        | _ => sorry
+    · intro h
+      induction l with
+        | true =>
+          cases b with
+            | true => exact LogicEval.true
+            | false => contradiction
+        | false =>
+          cases b with
+            | true => contradiction
+            | false => exact LogicEval.false
+        | eq e₁ e₂ => sorry
+        -- Other Arith cases
+        | not e ih => sorry
+        | and e₁ e₂ ih₁ ih₂ => sorry
+        | _ => sorry
+end AExp
+
+namespace Division
+  inductive Arith: Type where
+    | num (n: Nat): Arith
+    | plus (e₁ e₂: Arith): Arith
+    | minus (e₁ e₂: Arith): Arith
+    | mult (e₁ e₂: Arith): Arith
+    | div (e₁ e₂: Arith): Arith
+
+  inductive ArithEval: Arith → Nat → Prop where
+    | num (n: Nat): ArithEval (.num n) n
+    | plus (e₁ e₂: Arith) (n₁ n₂: Nat) (h₁: ArithEval e₁ n₁) (h₂: ArithEval e₂ n₂): ArithEval (.plus e₁ e₂) (n₁ + n₂)
+    | minus (e₁ e₂: Arith) (n₁ n₂: Nat) (h₁: ArithEval e₁ n₁) (h₂: ArithEval e₂ n₂): ArithEval (.minus e₁ e₂) (n₁ - n₂)
+    | mult (e₁ e₂: Arith) (n₁ n₂: Nat) (h₁: ArithEval e₁ n₁) (h₂: ArithEval e₂ n₂): ArithEval (.mult e₁ e₂) (n₁ * n₂)
+    | div (e₁ e₂: Arith) (n₁ n₂ n₃: Nat) (nonZero: n₂ ≠ 0) (prod: n₂ * n₃ = n₁) (h₁: ArithEval e₁ n₁) (h₂: ArithEval e₂ n₂): ArithEval (.div e₁ e₂) n₃
+end Division
+
+namespace Any
+  inductive Arith: Type where
+    | any: Arith
+    | num (n: Nat): Arith
+    | plus (e₁ e₂: Arith): Arith
+    | minus (e₁ e₂: Arith): Arith
+    | mult (e₁ e₂: Arith): Arith
+
+  inductive ArithEval: Arith → Nat → Prop where
+    | any (n: Nat): ArithEval .any n
+    | num (n: Nat): ArithEval (.num n) n
+    | plus (e₁ e₂: Arith) (n₁ n₂: Nat) (h₁: ArithEval e₁ n₁) (h₂: ArithEval e₂ n₂): ArithEval (.plus e₁ e₂) (n₁ + n₂)
+    | minus (e₁ e₂: Arith) (n₁ n₂: Nat) (h₁: ArithEval e₁ n₁) (h₂: ArithEval e₂ n₂): ArithEval (.minus e₁ e₂) (n₁ - n₂)
+    | mult (e₁ e₂: Arith) (n₁ n₂: Nat) (h₁: ArithEval e₁ n₁) (h₂: ArithEval e₂ n₂): ArithEval (.mult e₁ e₂) (n₁ * n₂)
+end Any
+
+/-
+## Expressions with Variables
+-/
+
+def State: Type := TotalMap Nat
+
+def State.empty: State := TotalMap.empty 0
+
+def State.build (l: List (String × Nat)): State :=
+  fold State.empty l
+  where
+    fold (s: State): List (String × Nat) → State
+      | [] => s
+      | (k, v) :: tl => fold (s.update k v) tl
+
+inductive Arith: Type where
+  | num (n: Nat): Arith
+  | ident (id: String): Arith
+  | plus (e₁ e₂: Arith): Arith
+  | minus (e₁ e₂: Arith): Arith
+  | mult (e₁ e₂: Arith): Arith
+
+inductive Logic: Type where
+  | true: Logic
+  | false: Logic
+  | eq (e₁ e₂: Arith): Logic
+  | neq (e₁ e₂: Arith): Logic
+  | le (e₁ e₂: Arith): Logic
+  | gt (e₁ e₂: Arith): Logic
+  | not (e: Logic): Logic
+  | and (e₁ e₂: Logic): Logic
+
+/-
+### Notations
+-/
+
+-- TODO: Implement syntax extensions (https://leanprover.github.io/lean4/doc/macro_overview.html)
+
+instance: Coe Bool Logic where
+  coe: Bool → Logic
+    | true => Logic.true
+    | false => Logic.false
+instance: Coe Nat Arith where
+  coe n := Arith.num n
+instance: OfNat Arith n where
+  ofNat := Arith.num n
+instance: Coe String Arith where
+  coe id := Arith.ident id
+
+instance: Add Arith where
+  add x y := Arith.plus x y
+instance: Sub Arith where
+  sub x y := Arith.minus x y
+instance: Mul Arith where
+  mul x y := Arith.mult x y
+
+instance: Neg Logic where
+  neg x := Logic.not x
+
+/-
+### Evaluation
+-/
+
+def Arith.eval (state: State): Arith → Nat
+  | num n => n
+  | ident id => state id
+  | plus e₁ e₂ => (e₁.eval state) + (e₂.eval state)
+  | minus e₁ e₂ => (e₁.eval state) - (e₂.eval state)
+  | mult e₁ e₂ => (e₁.eval state) * (e₂.eval state)
+
+def Logic.eval (state: State): Logic → Bool
+  | true => Bool.true
+  | false => Bool.false
+  | eq e₁ e₂ => (e₁.eval state) == (e₂.eval state)
+  | neq e₁ e₂ => (e₁.eval state) != (e₂.eval state)
+  | le e₁ e₂ => (e₁.eval state) ≤ (e₂.eval state)
+  | gt e₁ e₂ => (e₁.eval state) > (e₂.eval state)
+  | not e => !(e.eval state)
+  | and e₁ e₂ => (e₁.eval state) && (e₂.eval state)
+
+example: ((3: Arith) + "X" * 2).eval (State.build [("X", 5)]) = 13 := rfl
+example: (("Z": Arith) + "X" * "Y").eval (State.build [("X", 5), ("Y", 4)]) = 20 := rfl
+example: (Logic.and true (.not (.le "X" 4))).eval (State.build [("X", 5)]) = true := rfl
+
+/-
+## Commands
+-/
+
+inductive Command: Type where
+  | skip: Command
+  | assign (id: String) (e: Arith): Command
+  | seq (c₁ c₂: Command): Command
+  | if (b: Logic) (c₁ c₂: Command): Command
+  | while (b: Logic) (c: Command): Command
+
+instance: Coe (List Command) Command where
+  coe l :=
+    let rec conv: List Command → Command
+      | [] => .skip
+      | hd::[] => hd
+      | hd::tl => .seq hd (conv tl)
+    conv l
+
+def factorial: Command :=
+  [
+    (Command.assign "Z" "X"),
+    (.assign "Y" 1),
+    (.while (.neq "Z" 0) [
+      (Command.assign "Y" ("Y" * "Z")),
+      (.assign "Z" ("Z" - 1))
+    ])
+  ]
+
+/-
+### Desugaring Notations
+-/
+
+set_option pp.notation true
+set_option pp.coercions false
+
+#print factorial
+
+set_option pp.notation false
+set_option pp.coercions true
+
+/-
+### Locate, Again
+-/
+
+-- Appears to be Coq specific
+
+/- #### Finding Identifiers -/
+/- #### Finding Notations -/
+
+/-
+### More Examples
+-/
+
+section
+  /- #### Assignment -/
+
+  def plus2: Command := .assign "X" ("X" + 2)
+  def xTimesYInZ: Command := .assign "Z" ("X" * "Y")
+
+  /- #### Loops -/
+
+  private def subtractSlowlyBody: Command := ([
+    (.assign "Z" ("Z" - 1)),
+    (.assign "X" ("X" - 1))
+  ]: List Command)
+
+  private def subtractSlowly: Command :=
+    .while (.neq "X" 0) subtractSlowlyBody
+
+  private def subtract3From5Slowly: Command := ([
+    (.assign "X" 3),
+    (.assign "Z" 5),
+    subtractSlowly
+  ]: List Command)
+
+  /- #### An Infinite Loop -/
+
+  def loopForever: Command := .while .true .skip
+end
+
+/-
+## Evaluating Commands
+-/
+
+def Command.noBueno (state: State): Command → State
+  | .skip => state
+  | .assign id e => state.update id (e.eval state)
+  | .seq c₁ c₂ =>
+    state
+      |> c₁.noBueno
+      |> c₂.noBueno
+  | .if c t f =>
+    if c.eval state
+    then t.noBueno state
+    else f.noBueno state
+  | .while _ _ => state
+
+/-
+### Evaluation as a Relation
+-/
+
+inductive CommandEval: Command → State → State → Prop where
+  | skip (state: State): CommandEval .skip state state
+  | assign (state: State) (e: Arith) (n: Nat) (id: String) (h: e.eval state = n): CommandEval (.assign id e) state (state.update id n)
+  | seq (c₁ c₂: Command) (s₁ s₂ s₃: State) (h₁: CommandEval c₁ s₁ s₂) (h₂: CommandEval c₂ s₂ s₃): CommandEval (.seq c₁ c₂) s₁ s₃
+  | ifTrue (s₁ s₂: State) (c: Logic) (t f: Command) (h₁: c.eval s₁ = .true) (h₂: CommandEval t s₁ s₂): CommandEval (.if c t f) s₁ s₂
+  | ifFalse (s₁ s₂: State) (c: Logic) (t f: Command) (h₁: c.eval s₁ = .false) (h₂: CommandEval f s₁ s₂): CommandEval (.if c t f) s₁ s₂
+  | whileTrue (s₁ s₂ s₃: State) (c: Logic) (b: Command) (h₁: c.eval s₁ = .true) (h₂: CommandEval b s₁ s₂) (h₃: CommandEval (.while c b) s₂ s₃): CommandEval (.while c b) s₁ s₃
+  | whileFalse (c: Logic) (s: State) (b: Command) (h₁: c.eval s = .false): CommandEval (.while c b) s s
+
+def assignment (id: String) (n: Nat) (s: State): CommandEval (Command.assign id (n: Arith)) s (s.update id n) :=
+    have h: (n: Arith).eval s = n := by
+      unfold Arith.eval
+      rfl
+    CommandEval.assign s n n id h
+
+section
+  /- Useful definitions to save typing -/
+
+  private def x0: Command := .assign "X" 0
+  private def x2: Command := .assign "X" 2
+  private def y1: Command := .assign "Y" 1
+  private def y3: Command := .assign "Y" 3
+  private def z2: Command := .assign "Z" 2
+  private def z4: Command := .assign "Z" 4
+
+  private def xLe1: Logic := .le "X" 1
+
+  private def branch: Command := Command.if xLe1 y3 z4
+
+  /- Example -/
+
+  /- x := 2; if x ≤ 1 then y := 3 else z := 4 -/
+  example: CommandEval [x2, branch] State.empty (State.build [("X", 2), ("Z", 4)]) :=
+    let s₁: State := State.empty
+    let s₂: State := s₁.update "X" 2
+    let s₃: State := s₂.update "Z" 4
+
+    have h₁: CommandEval x2 s₁ s₂ := assignment "X" 2 s₁
+    have h₂: CommandEval branch s₂ s₃ :=
+      have h₁: (Logic.le "X" 1).eval s₂ = false := by
+        unfold Logic.eval
+        rfl
+      have h₂: CommandEval z4 s₂ s₃ := assignment "Z" 4 s₂
+      CommandEval.ifFalse s₂ s₃ xLe1 y3 z4 h₁ h₂
+
+    by
+      repeat unfold instCoeListCommand.conv
+      exact CommandEval.seq x2 branch s₁ s₂ s₃ h₁ h₂
+
+  /- x := 0; y := 1; z := 2 -/
+  example: CommandEval [x0, y1, z2] State.empty (State.build [("X", 0), ("Y", 1), ("Z", 2)]) :=
+    let s₁: State := State.empty
+    let s₂: State := s₁.update "X" 0
+    let s₃: State := s₂.update "Y" 1
+    let s₄: State := s₃.update "Z" 2
+
+    by
+      repeat unfold instCoeListCommand.conv
+      sorry
+
+  def sum: Command := sorry
+
+  example: CommandEval sum (State.build [("X", 2)]) (State.build [("X", 0), ("Y", 3), ("X", 1), ("Y", 2), ("Y", 0), ("X", 2)]) :=
+    sorry
+end
+
+/-
+### Determinism of Evaluation
+-/
+
+theorem CommandEval.deterministic (c: Command) (s₁ s₂ s₃: State) (h₁: CommandEval c s₁ s₂) (h₂: CommandEval c s₁ s₃): s₂ = s₃ := by
+  sorry
+
+/-
+## Reasoning about Imp Programs
+-/
+
+example (s₁ s₂: State) (n: Nat) (h₁: s₁ "X" = n) (h₂: CommandEval plus2 s₁ s₂): s₂ "X" = n + 2 := by
+  cases h₂ with
+    | assign _ _ n₁ _ h =>
+      rw [TotalMap.updateEq]
+      repeat unfold Arith.eval at h
+      rw [h₁] at h
+      apply Eq.symm
+      exact h
+
+example (s₁ s₂: State) (n₁ n₂: Nat) (h₁: s₁ "X" = n₁) (h₂: s₂ "Y" = n₂) (h₃: CommandEval xTimesYInZ s₁ s₂): s₂ "Y" = n₁ * n₂ := by
+  cases h₃ with
+    | assign _ _ n₃ _ h =>
+      simp_all
+      repeat unfold Arith.eval at h
+      repeat unfold Arith.eval at h
+      unfold TotalMap.update at h₂
+      simp_all
+      sorry
+
+example (s₁ s₂: State): ¬CommandEval loopForever s₁ s₂ := by
+  unfold Not
+  intro h
+  unfold loopForever at h
+  cases h with
+    | whileTrue _ s₃ _ _ _ h₁ h₂ h₃ => sorry
+    | whileFalse _ _ _ h₁ => contradiction
+
+def Command.noWhiles: Command → Bool
+  | .skip | .assign _ _ | .seq _ _ | .if _ _ _ => true
+  | _ => false
+
+inductive NoWhiles: Command → Prop where
+  | skip: NoWhiles .skip
+  | assign (id: String) (e: Arith): NoWhiles (.assign id e)
+  | seq (c₁ c₂: Command): NoWhiles (.seq c₁ c₂)
+  | if (c: Logic) (t f: Command): NoWhiles (.if c t f)
+
+theorem NoWhiles.noWhiles (c: Command): c.noWhiles = true ↔ NoWhiles c := by
+  sorry
+
+theorem CommandEval.noWhiles_terminate (s₁ s₂: State) (c: Command) (h: NoWhiles c): CommandEval c s₁ s₂ := by
+  sorry
+
+/-
+## Additional Exercises
+-/
+
+abbrev Stack: Type := List Nat
+
+def Stack.empty: Stack := []
+
+inductive StackInstr: Type where
+  | push (n: Nat): StackInstr
+  | load (id: String): StackInstr
+  | plus: StackInstr
+  | minus: StackInstr
+  | mult: StackInstr
+
+def StackInstr.eval (state: State): StackInstr → Stack → Stack
+  | .push n, stack => n :: stack
+  | .load id, stack => (state id) :: stack
+  | .plus, r :: l :: stack => (l + r) :: stack
+  | .minus, r :: l :: stack => (l - r) :: stack
+  | .mult, r :: l :: stack => (l * r) :: stack
+  | _, stack => stack
+
+abbrev Program: Type := List StackInstr
+
+def Program.eval (state: State) (program: Program) (init: Stack): Stack :=
+  program.foldl (fun stack instr => instr.eval state stack) init
+
+example: Program.eval State.empty [StackInstr.push 5, .push 3, .push 1, .minus] Stack.empty = [2, 5] := by rfl
+example: Program.eval (State.build [("X", 3)]) [StackInstr.push 4, .load "X", .mult, .plus] [3, 4] = [15, 4] := rfl
+
+def Arith.compile: Arith → Program
+  | .num n => [.push n]
+  | .ident id => [.load id]
+  | .plus e₁ e₂ => e₁.compile ++ e₂.compile ++ [.plus]
+  | .minus e₁ e₂ => e₁.compile ++ e₂.compile ++ [.minus]
+  | .mult e₁ e₂ => e₁.compile ++ e₂.compile ++ [.mult]
+
+example: (Arith.minus "X" (.mult 2 "Y")).compile = [StackInstr.load "X", .push 2, .load "Y", .mult, .minus] := rfl
+
+theorem eval_append (state: State) (p₁ p₂: Program) (stack: Stack): (p₁ ++ p₂).eval state stack = p₂.eval state (p₁.eval state stack) := by
+  sorry
+
+theorem Arith.compile.correct (state: State) (e: Arith): e.compile.eval state Stack.empty = [e.eval state] := by
+  sorry
+  where
+  helper (state: State) (stack: Stack) (e: Arith): e.compile.eval state stack = e.eval state :: stack := by
+    sorry
+
+def Logic.shortCircuitEval (state: State): Logic → Bool
+  | .and e₁ e₂ =>
+    if e₁.eval state
+    then Bool.true
+    else e₂.eval state
+  | l => l.eval state
+
+theorem Logic.shortCircuitEval.eval (state: State) (b: Logic): b.shortCircuitEval state = b.eval state := by
+  sorry
+
+namespace BreakImp
+  inductive Command: Type where
+    | skip: Command
+    | break: Command
+    | assign (id: String) (e: Arith): Command
+    | seq (c₁ c₂: Command): Command
+    | if (b: Logic) (c₁ c₂: Command): Command
+    | while (b: Logic) (c: Command): Command
+
+  inductive Result: Type where
+    | continue: Result
+    | break: Result
+
+  inductive CommandEval: Command → State → Result → State → Prop where
+    | skip (state: State): CommandEval .skip state .continue state
+    | break (state: State): CommandEval .break state .break state
+    | assign (state: State) (e: Arith) (n: Nat) (id: String) (h: e.eval state = n): CommandEval (.assign id e) state .continue (state.update id n)
+    | seq (c₁ c₂: Command) (s₁ s₂ s₃: State) (h₁: CommandEval c₁ s₁ .continue s₂) (h₂: CommandEval c₂ s₂ .continue s₃): CommandEval (.seq c₁ c₂) s₁ .continue s₃
+    | ifTrue (s₁ s₂: State) (c: Logic) (t f: Command) (h₁: c.eval s₁ = .true) (h₂: CommandEval t s₁ .continue s₂): CommandEval (.if c t f) s₁ .continue s₂
+    | ifFalse (s₁ s₂: State) (c: Logic) (t f: Command) (h₁: c.eval s₁ = .false) (h₂: CommandEval f s₁ .continue s₂): CommandEval (.if c t f) s₁ .continue s₂
+    | whileTrue (s₁ s₂ s₃: State) (c: Logic) (b: Command) (h₁: c.eval s₁ = .true) (h₂: CommandEval b s₁ .continue s₂) (h₃: CommandEval (.while c b) s₂ .continue s₃): CommandEval (.while c b) s₁ .continue s₃
+    | whileFalse (c: Logic) (s: State) (b: Command) (h₁: c.eval s = .false): CommandEval (.while c b) s .continue s
+
+  example (c: Command) (s₁ s₂: State) (r: Result): CommandEval (.seq .break c) s₁ r s₂ := by
+    sorry
+
+  example (c: Logic) (b: Command) (s₁ s₂: State) (r: Result): CommandEval (.while c b) s₁ r s₂ := by
+    sorry
+
+  example (c: Logic) (b: Command) (s₁ s₂: State) (h₁: c.eval s₁ = true) (h₂: CommandEval b s₁ .break s₂): CommandEval (.while c b) s₁ .continue s₂ := by
+    sorry
+
+  example (c₁ c₂: Command) (s₁ s₂ s₃: State) (h₁: CommandEval c₁ s₁ .continue s₂) (h₂: CommandEval c₂ s₂ .continue s₃): CommandEval (.seq c₁ c₂) s₁ .continue s₂ := by
+    sorry
+
+  example (c₁ c₂: Command) (s₁ s₂: State) (h₁: CommandEval c₁ s₁ .break s₂): CommandEval (.seq c₁ c₂) s₁ .break s₂ := by
+    sorry
+
+  example (c: Logic) (b: Command) (s₁ s₂: State) (h₁: CommandEval (.while c b) s₁ .continue s₂) (h₂: c.eval s₂ = true): ∃ s₃: State, CommandEval b s₃ .break s₂ := by
+    sorry
+
+  theorem CommandEval.deterministic (c: Command) (s₁ s₂ s₃: State) (r₁ r₂: Result) (h₁: CommandEval c s₁ r₁ s₂) (h₂: CommandEval c s₁ r₂ s₃): s₂ = s₃ ∧ r₁ = r₂ := by
+    sorry
+end BreakImp
+
+namespace ForImp
+  -- TODO
+end ForImp
