SoftwareFoundations/LogicalFoundations/ImpCEvalFun.lean
@@ -1,0 +1,6 @@
+/-
+# An Evaluation Function for Imp
+-/
+
+import «SoftwareFoundations».«LogicalFoundations».«Maps»
+import «SoftwareFoundations».«LogicalFoundations».«Imp»
