SoftwareFoundations/LogicalFoundations/ImpParser.lean
@@ -1,0 +1,5 @@
+/-
+# Lexing and Parsing in Lean
+-/
+
+import «SoftwareFoundations».«LogicalFoundations».«Maps»
