SoftwareFoundations/LogicalFoundations/Rel.lean
@@ -1,0 +1,232 @@
+/-
+# Properties of Relations
+-/
+
+/-
+## Relations
+-/
+
+def Relation (α: Type): Type := α → α → Prop
+
+inductive Le: Nat → Nat → Prop where
+  | eq (n: Nat): Le n n
+  | less (n₁ n₂: Nat) (h: Le n₁ n₂): Le n₁ n₂.succ
+
+#print Le
+#check (Le: Nat → Nat → Prop)
+#check (Le: Relation Nat)
+#check Le.recOn
+
+/-
+## Basic Properties
+-/
+
+/-
+### Partial Functions
+-/
+
+def PartialFunction (R: Relation α): Prop := ∀ x y₁ y₂: α, R x y₁ → R x y₂ → y₁ = y₂
+
+inductive NextNat: Relation Nat where
+  | next (n: Nat): NextNat n n.succ
+
+#check (NextNat: Relation Nat)
+
+theorem NextNat.partial_function: PartialFunction NextNat := by
+  unfold PartialFunction
+  intro x y₁ y₂ h₁ h₂
+  cases h₁ with
+    | next n₁ =>
+      cases h₂ with
+        | next n₂ => simp
+
+-- example: PartialFunction NextNat
+--   | x, y₁, .succ y₂, .next n₁, .next n₂ => sorry
+
+theorem Le.not_partial_function: ¬PartialFunction Le := by
+  unfold Not
+  unfold PartialFunction
+  intro h
+  have h₁: 0 = 1 := by
+    apply h 0
+    · exact Le.eq 0
+    · apply Le.less
+      · apply Le.eq
+  contradiction
+
+-- example: ¬PartialFunction Le :=
+--   fun h =>
+--     have h₃: 0 = 1 := h 0 0 1 Le.eq (Le.less 1 Le.eq)
+--     absurd (0 = 0) (0 = 1)
+
+namespace Duplicated
+  inductive TotalRelation: Nat → Nat → Prop where
+    | related (n₁ n₂: Nat): TotalRelation n₁ n₂
+
+  theorem TotalRelation.not_partial_function: ¬PartialFunction TotalRelation := by
+    unfold Not
+    unfold PartialFunction
+    intro h
+    have h₁: 0 = 1 := by
+      apply h 0
+      · exact TotalRelation.related 0 0
+      . exact TotalRelation.related 0 1
+    contradiction
+
+  example: ¬PartialFunction TotalRelation := sorry
+
+  inductive EmptyRelation: Nat → Nat → Prop
+
+  theorem EmptyRelation.partial_function: PartialFunction EmptyRelation := by
+    unfold PartialFunction
+    intro x y₁ y₂ h₁
+    cases h₁
+
+  -- example: PartialFunction EmptyRelation
+  --   | x, y₁, y₂, _, _ => sorry
+end Duplicated
+
+/-
+### Reflexive Relations
+-/
+
+def ReflexiveR (R: Relation α): Prop := ∀ x: α, R x x
+
+theorem Le.reflexive: ReflexiveR Le := by
+  unfold ReflexiveR
+  intro x
+  exact Le.eq x
+
+example: ReflexiveR Le
+  | n => Le.eq n
+
+/-
+### Transitive Relations
+-/
+
+def TransitiveR (R: Relation α): Prop := ∀ x₁ x₂ x₃: α, R x₁ x₂ → R x₂ x₃ → R x₁ x₃
+
+theorem Le.transitive: TransitiveR Le := by
+  unfold TransitiveR
+  intro x₁ x₂ x₃ h₁ h₂
+  induction h₁ with
+    | eq => exact h₂
+    | less n₁ h₃ ih =>
+      cases h₂ with
+        | eq => sorry
+        | less n₂ h₄ => sorry
+
+example: TransitiveR Le
+  | x₁, x₂, x₃, _, _ => sorry
+
+-- TODO: Extra theorems
+
+/-
+### Symmetric and Antisymmetric Relations
+-/
+
+def SymmetricR (R: Relation α): Prop := ∀ x₁ x₂: α, R x₁ x₂ → R x₂ x₁
+
+theorem Le.not_symmetric: ¬SymmetricR Le := by
+  unfold Not
+  unfold SymmetricR
+  intro h
+  have h₁: Le 1 0 :=
+    Le.eq 0
+      |> Le.less 0 0
+      |> h 0 1
+  contradiction
+
+example: ¬SymmetricR Le
+  | h =>
+    have h₁: Le 1 0 :=
+      Le.eq 0
+        |> Le.less 0 0
+        |> h 0 1
+    sorry
+
+def AntisymmetricR (R: Relation α): Prop := ∀ x₁ x₂: α, R x₁ x₂ → R x₂ x₁ → x₁ = x₂
+
+theorem Le.antisymmetric: AntisymmetricR Le := by
+  unfold AntisymmetricR
+  intro x₁ x₂ h₁ h₂
+  induction h₁ with
+    | eq => rfl
+    | less n₁ h₃ ih =>
+      cases h₂ with
+        | eq => rfl
+        | less n₂ h₄ => sorry
+
+example: AntisymmetricR Le
+  | x₁, x₂, h₁, h₂ => sorry
+
+-- TODO: Other examples
+
+/-
+### Equivalence Relations
+-/
+
+def EquivalenceR (R: Relation α): Prop := ReflexiveR R ∧ SymmetricR R ∧ TransitiveR R
+
+/-
+### Partial Orders and Preorders
+-/
+
+namespace Duplicated
+  def PartialOrder (R: Relation α): Prop := ReflexiveR R ∧ AntisymmetricR R ∧ TransitiveR R
+  def Preorder (R: Relation α): Prop := ReflexiveR R ∧ TransitiveR R
+
+  theorem Le.partial_order: PartialOrder Le := by
+    unfold PartialOrder
+    apply And.intro
+    · exact Le.reflexive
+    · apply And.intro
+      · exact Le.antisymmetric
+      · exact Le.transitive
+
+  example: PartialOrder Le :=
+    ⟨Le.reflexive, Le.antisymmetric, Le.transitive⟩
+end Duplicated
+
+/-
+## Reflexive Transitive Closure
+-/
+
+inductive RTC (R: Relation α): Relation α where
+  | base (x₁ x₂: α) (h: R x₁ x₂): RTC R x₁ x₂
+  | refl (x: α): RTC R x x
+  | trans (x₁ x₂ x₃: α) (h₁: RTC R x₁ x₂) (h₂: RTC R x₂ x₃): RTC R x₁ x₃
+
+theorem NextNat.rtc_le (n₁ n₂: Nat): Le n₁ n₂ ↔ RTC NextNat n₁ n₂ := by
+  apply Iff.intro
+  · intro h
+    induction h with
+      | eq => sorry
+      | less n h ih => sorry
+  · intro h
+    induction h with
+      | base x₁ x₂ h => sorry
+      | refl x => exact Le.eq x
+      | trans x₁ x₂ x₃ h₁ h₂ ih₁ ih₂ => sorry
+
+example (n₁ n₂: Nat): Le n₁ n₂ ↔ RTC NextNat n₁ n₂ :=
+  ⟨mp, mpr⟩
+  where
+    mp: Le n₁ n₂ → RTC NextNat n₁ n₂
+      | .eq _ => sorry
+      | .less _ _ h => sorry
+    mpr: RTC NextNat n₁ n₂ → Le n₁ n₂
+      | .base _ _ (.next _) => sorry -- Le.less n₁ n₂ (Le.eq n₁ n₁)
+      | .refl _ => Le.eq n₁
+      | .trans _ _ _ h₁ h₂ => sorry
+
+/-
+Lean doesn't allow this type of inductive definition, while Coq does.  The
+remaining exercies are therefore moot.
+-/
+-- inductive RTC₂ (R: Relation α) (x: α): α → Prop where
+--   | refl: RTC₂ R x x
+--   | trans (x₁ x₂: α) (h₁: R x x₁) (h₂: RTC₂ R x x₁) (h₃: RTC₂ R x₁ x₂): RTC₂ R x x₂
+
+-- Just to have something after the comment to make the parser happy
+#check Nat
